fix semax_ext

veric/semax_ext.v
@@ -94,9 +94,9 @@ Proof.
   intros; repeat (apply eq_dec || decide equality).
 Qed.
 
-Definition funspec2pre' (A : TypeTree) (P: dtfr (ArgsTT A)) (x : (nat * iResUR Σ * ofe_car (dtfr A))%type) (ge_s: injective_PTree block) sig args z m :=
+Definition funspec2pre' (A : TypeTree) (P: dtfr (ArgsTT A)) (x : (nat * iResUR Σ * ofe_car (dtfr A))%type) sig args z m :=
   let '(n, phi, x') := x in ✓{n} phi /\ Val.has_type_list args sig /\
-    ouPred_holds (state_interp m z ∗ P x' (filter_genv (symb2genv ge_s), args)) n phi.
+    ouPred_holds (state_interp m z ∗ P x' args) n phi.
 
 Definition funspec2pre (ext_link: Strings.String.string -> ident) (A : TypeTree)
   (P: dtfr (ArgsTT A))
@@ -105,12 +105,12 @@ Definition funspec2pre (ext_link: Strings.String.string -> ident) (A : TypeTree)
   match oi_eq_dec (Some (id, sig)) (ef_id_sig ext_link ef) as s
   return ((if s then (nat * iResUR Σ * ofe_car (dtfr A))%type else ext_spec_type Espec ef) -> Prop)
   with
-    | left _ => fun x => funspec2pre' A P x ge_s (map proj_xtype (sig_args (ef_sig ef))) args z m
+    | left _ => fun x => funspec2pre' A P x (map proj_xtype (sig_args (ef_sig ef))) args z m
     | right n => fun x' => ext_spec_pre Espec ef x' ge_s tys args z m
   end x.
 
-Definition funspec2post' (A : TypeTree) (Q: dtfr (AssertTT A)) (x : (nat * iResUR Σ * ofe_car (dtfr A))%type) (ge_s: injective_PTree block) tret ret z m :=
-  let '(n, phi, x') := x in ouPred_holds (|==> state_interp m z ∗ Q x' (make_ext_rval (filter_genv (symb2genv ge_s)) tret ret)) n phi.
+Definition funspec2post' (A : TypeTree) (Q: dtfr (AssertTT A)) (x : (nat * iResUR Σ * ofe_car (dtfr A))%type) tret ret z m :=
+  let '(n, phi, x') := x in ouPred_holds (|==> state_interp m z ∗ Q x' (make_ext_rval tret ret)) n phi.
 
 Definition funspec2post (ext_link: Strings.String.string -> ident) (A : TypeTree)
   (Q: dtfr (AssertTT A))
@@ -118,7 +118,7 @@ Definition funspec2post (ext_link: Strings.String.string -> ident) (A : TypeTree
   match oi_eq_dec (Some (id, sig)) (ef_id_sig ext_link ef) as s
   return ((if s then (nat * iResUR Σ * ofe_car (dtfr A))%type else ext_spec_type Espec ef) -> Prop)
   with
-    | left _ => fun x => funspec2post' A Q x ge_s tret ret z m
+    | left _ => fun x => funspec2post' A Q x tret ret z m
     | right n => fun x' => ext_spec_post Espec ef x' ge_s tret ret z m
   end x.
 
@@ -139,23 +139,22 @@ Definition wf_funspec (f : funspec) :=
     | mk_funspec sig cc E A P Q =>
         forall a (ge ge': genv) args,
           Genv.genv_symb ge = Genv.genv_symb ge' ->
-          P a (filter_genv ge, args) 
-         ⊢ P a (filter_genv ge', args)
+          P a args 
+         ⊢ P a args
   end.
 
-Lemma make_ext_args_filtergenv (ge ge' : genv)
+(* Lemma make_ext_args_filtergenv (ge ge' : genv)
       (H: Genv.genv_symb ge = Genv.genv_symb ge'):
   filter_genv ge = filter_genv ge'.
 Proof.
 intros.
 unfold filter_genv, Genv.find_symbol.
 rewrite H; auto.
-Qed.
+Qed. *)
 
 Lemma all_funspecs_wf f : wf_funspec f.
 Proof.
-destruct f; simpl; intros a ge ge' args H.
-erewrite make_ext_args_filtergenv; eauto.
+destruct f; simpl; intros a ge ge' args H. done.
 Qed.
 
 #[local] Obligation Tactic := idtac.
@@ -180,7 +179,7 @@ Lemma add_funspecs_pre (ext_link: Strings.String.string -> ident)
   funspecs_norepeat fs ->
   In (ext_link id, (mk_funspec sig cc A E P Q)) fs -> ∃ H : ext_spec_type (add_funspecs_rec ext_link Espec fs) ef = (nat * iResUR Σ * dtfr A)%type,
   ext_spec_pre (add_funspecs_rec ext_link Espec fs) ef x ge_s tys args z m =
-  funspec2pre' A P (eq_rect _ Datatypes.id x _ H) ge_s (map proj_xtype (sig_args (ef_sig ef))) args z m.
+  funspec2pre' A P (eq_rect _ Datatypes.id x _ H) (map proj_xtype (sig_args (ef_sig ef))) args z m.
 Proof.
   induction fs; [intros; exfalso; auto|]; intros ?? [-> | H1]; simpl in *.
   - clear IHfs H; unfold funspec2jspec; simpl.
@@ -203,7 +202,7 @@ Lemma add_funspecs_post (ext_link: Strings.String.string -> ident)
   funspecs_norepeat fs ->
   In (ext_link id, (mk_funspec sig cc A E P Q)) fs -> ∃ H : ext_spec_type (add_funspecs_rec ext_link Espec fs) ef = (nat * iResUR Σ * dtfr A)%type,
   ext_spec_post (add_funspecs_rec ext_link Espec fs) ef x ge_s ty v z m =
-  funspec2post' A Q (eq_rect _ Datatypes.id x _ H) ge_s ty v z m.
+  funspec2post' A Q (eq_rect _ Datatypes.id x _ H) ty v z m.
 Proof.
   induction fs; [intros; exfalso; auto|]; intros ?? [-> | H1]; simpl in *.
   - clear IHfs H; unfold funspec2jspec; simpl.
@@ -226,12 +225,12 @@ Lemma add_funspecs_prepost (ext_link: Strings.String.string -> ident)
   funspecs_norepeat fs ->
   In (ext_link id, (mk_funspec sig cc A E P Q)) fs ->
   forall md z, ⌜Val.has_type_list args (map proj_xtype (sig_args (ef_sig ef)))⌝ ∧
-        state_interp md z ∗ P x (filter_genv (symb2genv ge_s), args) ⊢
+        state_interp md z ∗ P x args ⊢
   ∃ x' : ext_spec_type (add_funspecs_rec ext_link Espec fs) ef,
     ⌜ext_spec_pre (add_funspecs_rec ext_link Espec fs) ef x' ge_s tys args z md⌝ ∧
     (∀ (tret : xtype) (ret : option val) (m' : Memory.mem) z',
        ⌜ext_spec_post (add_funspecs_rec ext_link Espec fs) ef x' ge_s tret ret z' m'⌝
-       → |==> state_interp m' z' ∗ ofe_mor_car _ _ Q x (make_ext_rval (filter_genv (symb2genv ge_s)) tret ret)).
+       → |==> state_interp m' z' ∗ ofe_mor_car _ _ Q x (make_ext_rval tret ret)).
 Proof.
 induction fs; [intros; exfalso; auto|]; intros ef H H1 md z.
 destruct H1 as [H1|H1].
@@ -276,12 +275,12 @@ Lemma add_funspecs_prepost_void  (ext_link: Strings.String.string -> ident)
   funspecs_norepeat fs ->
   In (ext_link id, (mk_funspec (sig, tvoid) cc A E P Q)) fs ->
   forall md z, ⌜Val.has_type_list args (map proj_xtype (sig_args (ef_sig ef)))⌝ ∧
-        state_interp md z ∗ P x (filter_genv (symb2genv ge_s), args) ⊢
+        state_interp md z ∗ P x args ⊢
   ∃ x' : ext_spec_type (add_funspecs_rec ext_link Espec fs) ef,
     ⌜ext_spec_pre (add_funspecs_rec ext_link Espec fs) ef x' ge_s tys args z md⌝ ∧
     (∀ (tret : xtype) (ret : option val) (m' : Memory.mem) z',
        ⌜ext_spec_post (add_funspecs_rec ext_link Espec fs) ef x' ge_s tret ret z' m'⌝
-       → |==> state_interp m' z' ∗ ofe_mor_car _ _ Q x (make_ext_rval (filter_genv (symb2genv ge_s)) tret ret)).
+       → |==> state_interp m' z' ∗ ofe_mor_car _ _ Q x (make_ext_rval tret ret)).
 Proof.
   apply add_funspecs_prepost.
 Qed.
